Continue cleaning code up

CodeGen.v
@@ -10,228 +10,21 @@ Require Import Loop.
 Require Import PolyLoop.
 Require Import PolyLang.
 Require Import Misc.
+Require Import Semantics.
 Require Import Instr.
 Require Import VplInterface.
 Require Import Result.
 Require Import Canonizer.
 Require Import Heuristics.
 Require Import Projection.
+Require Import TopoSort.
+Require Import LoopGen.
 
 Require Import Vpl.Impure.
 Require Import ImpureAlarmConfig.
 
 Open Scope Z_scope.
 Open Scope list_scope.
-
-(** * Creating expressions that evaluate to a given linear function *)
-
-
-Fixpoint make_linear_expr (n : nat) (l : list Z) :=
-  match n, l with
-  | O, _ | _, nil => Constant 0
-  | S n, x :: l => make_sum (make_mult x (Var n)) (make_linear_expr n l)
-  end.
-
-Theorem make_linear_expr_correct_aux :
-  forall n l env, (length env >= n)%nat -> eval_expr env (make_linear_expr n l) = dot_product l (rev (firstn n env)).
-Proof.
-  induction n.
-  - intros l env Hel. destruct env; destruct l; simpl in *; auto; lia.
-  - intros l env Hel.
-    destruct l as [|x l]; simpl in Hel; destruct (rev (firstn (S n) env)) as [|y ev] eqn:Hrev; auto; simpl; auto.
-    + destruct env as [|e env]; simpl in *; [lia | destruct (rev (firstn n env)); simpl in *; congruence].
-    + rewrite firstn_nth_app with (d := 0) in Hrev by auto. rewrite rev_unit in Hrev.
-      injection Hrev as Hnth Hrev. rewrite make_sum_correct, make_mult_correct, IHn by lia; simpl. congruence.
-Qed.
-
-Theorem make_linear_expr_correct :
-  forall n l env, length env = n -> eval_expr env (make_linear_expr n l) = dot_product l (rev env).
-Proof.
-  intros. rewrite make_linear_expr_correct_aux by lia. f_equal. f_equal. apply firstn_all2. lia.
-Qed.
-
-Definition make_affine_expr (n : nat) (e : (list Z * Z)%type) := make_sum (make_linear_expr n (fst e)) (Constant (snd e)).
-
-Theorem make_affine_expr_correct :
-  forall n e env, length env = n -> eval_expr env (make_affine_expr n e) = dot_product (fst e) (rev env) + snd e.
-Proof.
-  intros. unfold make_affine_expr. rewrite make_sum_correct, make_linear_expr_correct; auto.
-Qed.
-
-(** * Creating upper and lower bounds for a given variable in a constraint *)
-
-Definition make_lower_bound n c :=
-  make_div (make_sum (Constant ((- nth n (fst c) 0) - 1)) (make_affine_expr n (fst c, -(snd c)))) (-(nth n (fst c) 0)).
-
-Lemma make_lower_bound_correct :
-  forall n c env x, length env = n -> nth n (fst c) 0 < 0 -> (eval_expr env (make_lower_bound n c) <= x <-> satisfies_constraint (rev env ++ x :: nil) c = true).
-Proof.
-  intros n c env x Hlen Hneg.
-  unfold satisfies_constraint. simpl.
-  reflect. unfold make_lower_bound; rewrite make_div_correct, make_sum_correct, make_affine_expr_correct by auto. simpl.
-  rewrite dot_product_app_left, dot_product_resize_right, dot_product_commutative.
-  rewrite rev_length, Hlen.
-  replace (dot_product (x :: nil) (skipn n (fst c))) with (x * nth n (fst c) 0) at 1;
-    [| transitivity (x * nth 0 (skipn n (fst c)) 0);
-       [ rewrite nth_skipn; f_equal; f_equal; lia
-       | destruct (skipn n (fst c)) as [|z l]; [|destruct l]; simpl; lia
-       ]
-    ].
-  rewrite div_le_iff by lia. nia.
-Qed.
-
-Definition make_upper_bound n c :=
-  make_div (make_sum (Constant (nth n (fst c) 0)) (make_affine_expr n (mult_vector (-1) (fst c), snd c))) (nth n (fst c) 0).
-
-Lemma make_upper_bound_correct :
-  forall n c env x, length env = n -> 0 < nth n (fst c) 0 -> (x < eval_expr env (make_upper_bound n c) <-> satisfies_constraint (rev env ++ x :: nil) c = true).
-Proof.
-  intros n c env x Hlen Hpos.
-  unfold satisfies_constraint. simpl.
-  reflect. unfold make_upper_bound; rewrite make_div_correct, make_sum_correct, make_affine_expr_correct by auto. simpl.
-  rewrite dot_product_mult_left.
-  rewrite dot_product_app_left, dot_product_resize_right, dot_product_commutative.
-  rewrite rev_length, Hlen.
-  replace (dot_product (x :: nil) (skipn n (fst c))) with (x * nth n (fst c) 0) at 1;
-    [| transitivity (x * nth 0 (skipn n (fst c)) 0);
-       [ rewrite nth_skipn; f_equal; f_equal; lia
-       | destruct (skipn n (fst c)) as [|z l]; [|destruct l]; simpl; lia
-       ]
-    ].
-  rewrite div_gt_iff by lia. nia.
-Qed.
-
-Opaque make_lower_bound make_upper_bound.
-
-(** * Finding the upper and lower bounds for a given variable of a polyhedron *)
-
-Fixpoint find_lower_bound_aux (e : option expr) (n : nat) (p : polyhedron) :=
-  match p with
-  | nil => match e with Some e => Ok e | None => Err "No lower bound found" end
-  | c :: p => if nth n (fst c) 0 <? 0 then
-               find_lower_bound_aux (Some (match e with Some e => make_max e (make_lower_bound n c) | None => make_lower_bound n c end)) n p
-             else
-               find_lower_bound_aux e n p
-  end.
-
-Lemma find_lower_bound_aux_correct :
-  forall n pol env x e lb, find_lower_bound_aux e n pol = Ok lb -> length env = n ->
-                      eval_expr env lb <= x <->
-                      ((match e with Some e => eval_expr env e <= x | None => True end) /\
-                       forall c, In c pol -> nth n (fst c) 0 < 0 -> satisfies_constraint (rev env ++ x :: nil) c = true).
-Proof.
-  intros n pol. induction pol.
-  - intros env x e lb Hlb Hlength. simpl in *.
-    destruct e; simpl in *; [|congruence].
-    injection Hlb as Hlb; rewrite Hlb.
-    split; intros H; tauto.
-  - intros env x e lb Hlb Hlen. simpl in *.
-    destruct (nth n (fst a) 0 <? 0) eqn:Hcmp.
-    + reflect. rewrite IHpol; eauto; simpl.
-      destruct e; simpl; [rewrite make_max_correct, Z.max_lub_iff|]; rewrite make_lower_bound_correct by auto; split.
-      * intros [[H1 H2] H3]. split; auto. intros c [Hce|Hcin] Hcnth; [congruence|auto].
-      * intros [H1 H2]. split; [split|]; auto.
-      * intros [H1 H2]. split; auto. intros c [Hce|Hcin] Hcnth; [congruence|auto].
-      * intros [H1 H2]. split; auto.
-    + reflect. rewrite IHpol; eauto; simpl. f_equiv. split.
-      * intros H c [Hce|Hcin] Hcnth; auto; rewrite Hce in *; lia.
-      * intros H c Hcin Hcnth; auto.
-Qed.
-
-Fixpoint find_upper_bound_aux (e : option expr) (n : nat) (p : polyhedron) :=
-  match p with
-  | nil => match e with Some e => Ok e | None => Err "No upper bound found" end
-  | c :: p => if 0 <? nth n (fst c) 0 then
-               find_upper_bound_aux (Some (match e with Some e => make_min e (make_upper_bound n c) | None => make_upper_bound n c end)) n p
-             else
-               find_upper_bound_aux e n p
-  end.
-
-Lemma find_upper_bound_aux_correct :
-  forall n pol env x e ub, find_upper_bound_aux e n pol = Ok ub -> length env = n ->
-                      x < eval_expr env ub <->
-                      ((match e with Some e => x < eval_expr env e | None => True end) /\
-                       forall c, In c pol -> 0 < nth n (fst c) 0 -> satisfies_constraint (rev env ++ x :: nil) c = true).
-Proof.
-  intros n pol. induction pol.
-  - intros env x e ub Hub Hlength. simpl in *.
-    destruct e; simpl in *; [|congruence].
-    injection Hub as Hub; rewrite Hub.
-    split; intros H; tauto.
-  - intros env x e lb Hub Hlen. simpl in *.
-    destruct (0 <? nth n (fst a) 0) eqn:Hcmp.
-    + reflect. rewrite IHpol; eauto; simpl.
-      destruct e; simpl; [rewrite make_min_correct, Z.min_glb_lt_iff|]; rewrite make_upper_bound_correct by auto; split.
-      * intros [[H1 H2] H3]. split; auto. intros c [Hce|Hcin] Hcnth; [congruence|auto].
-      * intros [H1 H2]. split; [split|]; auto.
-      * intros [H1 H2]. split; auto. intros c [Hce|Hcin] Hcnth; [congruence|auto].
-      * intros [H1 H2]. split; auto.
-    + reflect. rewrite IHpol; eauto; simpl. f_equiv. split.
-      * intros H c [Hce|Hcin] Hcnth; auto; rewrite Hce in *; lia.
-      * intros H c Hcin Hcnth; auto.
-Qed.
-
-Definition find_lower_bound := find_lower_bound_aux None.
-Definition find_upper_bound := find_upper_bound_aux None.
-
-Theorem find_lower_bound_correct :
-  forall n pol env x lb, find_lower_bound n pol = Ok lb -> length env = n ->
-                    eval_expr env lb <= x <-> (forall c, In c pol -> nth n (fst c) 0 < 0 -> satisfies_constraint (rev env ++ x :: nil) c = true).
-Proof.
-  intros n pol env x lb Hlb Hlen.
-  rewrite find_lower_bound_aux_correct by eauto. simpl. tauto.
-Qed.
-
-Theorem find_upper_bound_correct :
-  forall n pol env x ub, find_upper_bound n pol = Ok ub -> length env = n ->
-                    x < eval_expr env ub <-> (forall c, In c pol -> 0 < nth n (fst c) 0 -> satisfies_constraint (rev env ++ x :: nil) c = true).
-
-Proof.
-  intros n pol env x ub Hub Hlen.
-  rewrite find_upper_bound_aux_correct by eauto. simpl. tauto.
-Qed.
-
-Theorem find_bounds_correct :
-  forall n pol env x lb ub, find_lower_bound n pol = Ok lb -> find_upper_bound n pol = Ok ub -> length env = n ->
-                       eval_expr env lb <= x < eval_expr env ub <-> (forall c, In c pol -> nth n (fst c) 0 <> 0 -> satisfies_constraint (rev env ++ x :: nil) c = true).
-Proof.
-  intros n pol env x lb ub Hlb Hub Hlen.
-  rewrite find_lower_bound_correct; eauto.
-  rewrite find_upper_bound_correct; eauto.
-  split.
-  - intros [H1 H2] c Hin Hnotzero. destruct (nth n (fst c) 0 <=? 0) eqn:Hcmp; reflect; [apply H1 | apply H2]; auto; lia.
-  - intros H; split; intros c Hin Hcmp; apply H; auto; lia.
-Qed.
-
-
-Definition solve_eq n c :=
-  (make_div (make_affine_expr n (mult_vector (-1) (fst c), snd c)) (nth n (fst c) 0),
-   make_eq (make_mod (make_affine_expr n (mult_vector (-1) (fst c), snd c)) (nth n (fst c) 0)) (Constant 0)).
-
-Lemma solve_eq_correct :
-  forall n c env x, length env = n -> nth n (fst c) 0 <> 0 ->
-               (eval_expr env (fst (solve_eq n c)) = x /\ eval_test env (snd (solve_eq n c)) = true) <->
-                dot_product (rev env ++ x :: nil) (fst c) = snd c.
-Proof.
-  intros n c env x Hlen Hnz. simpl.
-  rewrite make_div_correct, make_eq_correct, make_mod_correct, !make_affine_expr_correct by auto. simpl.
-  rewrite !dot_product_mult_left, dot_product_app_left, dot_product_resize_right, dot_product_commutative.
-  rewrite rev_length, Hlen.
-  replace (dot_product (x :: nil) (skipn n (fst c))) with (x * nth n (fst c) 0) at 1;
-    [| transitivity (x * nth 0 (skipn n (fst c)) 0);
-       [ rewrite nth_skipn; f_equal; f_equal; lia
-       | destruct (skipn n (fst c)) as [|z l]; [|destruct l]; simpl; lia
-       ]
-    ].
-  reflect. split.
-  - intros [Hdiv Hmod]. rewrite <- Z.div_exact in Hmod by auto. nia.
-  - intros H. rewrite <- H, Z.add_assoc, Z.add_opp_diag_l, Z.add_0_l. split.
-    + apply Z.div_mul; auto.
-    + apply Z.mod_mul; auto.
-Qed.
-
-
-Parameter topo_sort_untrusted : list (list bool) -> imp (list nat).
 
 Definition isBottom pol :=
   BIND p <- lift (ExactCs.fromCs_unchecked (poly_to_Cs pol)) -; lift (CstrDomain.isBottom p).
@@ -325,36 +118,12 @@ Qed.
 
 Module Proj := FourierMotzkinProject CoreAlarmed.
 Module Canon := VplCanonizer.
-Module PO := PolyProjectImpl CoreAlarmed Canon Proj.
-Import PO.
+Module PPI := PolyProjectImpl CoreAlarmed Canon Proj.
+Import PPI.
 
 Global Opaque project.
 
 (** * Generating the code *)
-
-Definition res_to_alarm {A : Type} (d : A) (x : result A) : imp A :=
-  match x with
-  | Ok a => pure a
-  | Err s => alarm s d
-  end.
-
-Lemma res_to_alarm_correct :
-  forall (A : Type) (d : A) (x : result A) (y : A),
-    mayReturn (res_to_alarm d x) y -> x = Ok y.
-Proof.
-  intros A d x y. destruct x; simpl.
-  - intros H. f_equal. apply mayReturn_pure. auto.
-  - intros H. apply mayReturn_alarm in H. tauto.
-Qed.
-
-Definition make_affine_test n c := make_le (make_linear_expr n (fst c)) (Constant (snd c)).
-
-Lemma make_affine_test_correct :
-  forall env n c, length env = n -> eval_test env (make_affine_test n c) = satisfies_constraint (rev env) c.
-Proof.
-  intros. simpl in *. unfold make_affine_test. rewrite make_le_correct, make_linear_expr_correct; auto.
-  rewrite dot_product_commutative. reflexivity.
-Qed.
 
 Fixpoint sequence {A : Type} (l : list (imp A)) : imp (list A) :=
   match l with
@@ -364,188 +133,6 @@ Fixpoint sequence {A : Type} (l : list (imp A)) : imp (list A) :=
 
 Definition fmap {A B : Type} (f : A -> B) (x : imp A) : imp B :=
   BIND y <- x -; pure (f y).
-
-Definition make_poly_test n poly :=
-  and_all (map (make_affine_test n) poly).
-
-Lemma make_poly_test_correct :
-  forall n poly env, length env = n ->
-                eval_test env (make_poly_test n poly) = in_poly (rev env) poly.
-Proof.
-  intros n poly env Hlen.
-  unfold make_poly_test. rewrite and_all_correct. unfold in_poly.
-  rewrite forallb_map. apply forallb_ext. intros c. apply make_affine_test_correct. auto.
-Qed.
-
-Definition scan_dimension (n : nat) (inner : stmt) (p : polyhedron) : imp stmt :=
-  match find_eq n p with
-  | Some c =>
-    let '(result, test) := solve_eq n c in
-    let cstrs := map (fun c1 => make_affine_test n (make_constraint_with_eq n c c1)) (filter (fun c => negb (nth n (fst c) 0 =? 0)) p) in
-    let cstrs1 := map (make_affine_test n) (filter (fun c => nth n (fst c) 0 =? 0) p) in
-    pure (make_guard (make_and test (and_all (cstrs ++ cstrs1))) (make_let result inner))
-  | None =>
-    BIND lb <- res_to_alarm (Constant 0) (find_lower_bound n p) -;
-    BIND ub <- res_to_alarm (Constant 0) (find_upper_bound n p) -;
-    let cstrs := filter (fun c => nth n (fst c) 0 =? 0) p in
-    pure (make_guard (make_poly_test n cstrs) (Loop lb ub inner))
-  end.
-
-Lemma dot_product_nth_zero_eval :
-  forall env n u x, nth n u 0 = 0 -> length env = n -> dot_product (env ++ x :: nil) u = dot_product env u.
-Proof.
-  intros env n u x H1 H2.
-  rewrite <- dot_product_assign_left_zero with (k := n) (s := 0) by auto.
-  rewrite assign_app_ge by lia. rewrite H2, Nat.sub_diag.
-  unfold assign. simpl.
-  f_equiv. rewrite <- app_nil_r. f_equiv.
-Qed.
-
-Lemma satisfies_constraint_nth_zero_eq :
-  forall env n c x, nth n (fst c) 0 = 0 -> length env = n -> satisfies_constraint (env ++ x :: nil) c = satisfies_constraint env c.
-Proof.
-  intros. unfold satisfies_constraint.
-  erewrite dot_product_nth_zero_eval; eauto.
-Qed.
-
-Lemma scan_dimension_sem :
-  forall n inner pol,
-    WHEN st <- scan_dimension n inner pol THEN
-         forall env mem1 mem2,
-           length env = n ->
-           exists lb ub,
-             (loop_semantics st env mem1 mem2 <-> iter_semantics (fun x => loop_semantics inner (x :: env)) (Zrange lb ub) mem1 mem2) /\
-             (forall x, in_poly (rev (x :: env)) pol = true <-> lb <= x < ub).
-Proof.
-  intros n inner pol st Hst env mem1 mem2 Henvlen.
-  unfold scan_dimension in Hst.
-  destruct (find_eq n pol) as [c|] eqn:Hfindeq.
-  - destruct (solve_eq n c) as [result test] eqn:Hsolve. apply mayReturn_pure in Hst; rewrite <- Hst.
-    match goal with [ Hst : make_guard ?T _ = _ |- _ ] => set (test1 := T) end.
-    assert (Hcnth : 0 < nth n (fst c) 0) by (eapply find_eq_nth; eauto).
-    destruct (eval_test env test1) eqn:Htest1.
-    + exists (eval_expr env result). exists (eval_expr env (Sum result (Constant 1))). split.
-      * split.
-        -- intros Hsem. rewrite make_guard_correct, Htest1 in Hsem. unfold make_let in Hsem. inversion_clear Hsem. auto.
-        -- intros Hsem. rewrite make_guard_correct, Htest1. unfold make_let. constructor; auto.
-      * intros x. simpl.
-        unfold test1 in Htest1. rewrite make_and_correct in Htest1; reflect.
-        rewrite and_all_correct in Htest1. destruct Htest1 as [Htest Hcstr].
-        rewrite forallb_app, andb_true_iff in Hcstr. destruct Hcstr as [Hcstr1 Hcstr2].
-        transitivity (eval_expr env (fst (solve_eq n c)) = x /\ eval_test env (snd (solve_eq n c)) = true); [|rewrite Hsolve; simpl; intuition lia].
-        rewrite solve_eq_correct by (auto || lia).
-        split.
-        -- intros H. unfold in_poly in H. rewrite forallb_forall in H.
-           eapply find_eq_correct_1; eauto.
-        -- intros H. unfold in_poly; rewrite forallb_forall. intros c1 Hc1in.
-           rewrite forallb_map, forallb_forall in Hcstr1, Hcstr2. specialize (Hcstr1 c1). specialize (Hcstr2 c1).
-           rewrite filter_In, make_affine_test_correct in Hcstr1, Hcstr2 by auto.
-           destruct (nth n (fst c1) 0 =? 0) eqn:Hc1nth; reflect.
-           ++ erewrite satisfies_constraint_nth_zero_eq; rewrite ?rev_length; eauto.
-           ++ rewrite <- make_constraint_with_eq_correct_1 with (n := n) (c1 := c) by (auto || lia).
-              erewrite satisfies_constraint_nth_zero_eq; rewrite ?rev_length; eauto.
-              apply make_constraint_with_eq_nth; lia.
-    + exists 0. exists 0. split.
-      * split.
-        -- intros Hsem. rewrite make_guard_correct, Htest1 in Hsem; rewrite Hsem. constructor; lia.
-        -- intros Hsem. rewrite make_guard_correct, Htest1. inversion_clear Hsem. reflexivity.
-      * split; [|lia]. intros H. exfalso.
-        enough (eval_test env test1 = true) by congruence.
-        unfold test1. rewrite make_and_correct, and_all_correct, forallb_app, !forallb_map. reflect.
-        unfold in_poly in H. rewrite forallb_forall in H.
-        assert (Heq : dot_product (rev (x :: env)) (fst c) = snd c) by (eapply find_eq_correct_1; eauto). simpl in Heq.
-        split; [|split].
-        -- rewrite <- solve_eq_correct in Heq; [|exact Henvlen|lia]. rewrite Hsolve in Heq; simpl in Heq; tauto.
-        -- rewrite forallb_forall. intros c1 Hc1in. rewrite filter_In in Hc1in. reflect.
-           rewrite make_affine_test_correct by auto. destruct Hc1in as [Hc1in Hc1n]. specialize (H c1 Hc1in).
-           rewrite <- make_constraint_with_eq_correct_1 with (n := n) (c1 := c) in H by (auto || lia).
-           simpl in H; erewrite satisfies_constraint_nth_zero_eq in H; rewrite ?rev_length; eauto.
-           apply make_constraint_with_eq_nth; lia.
-        -- rewrite forallb_forall. intros c1 Hc1in. rewrite filter_In in Hc1in. reflect.
-           rewrite make_affine_test_correct by auto. destruct Hc1in as [Hc1in Hc1n]. specialize (H c1 Hc1in).
-           simpl in H; erewrite satisfies_constraint_nth_zero_eq in H; rewrite ?rev_length; eauto.
-  - bind_imp_destruct Hst lb Hlb. apply res_to_alarm_correct in Hlb.
-    bind_imp_destruct Hst ub Hub. apply res_to_alarm_correct in Hub.
-    apply mayReturn_pure in Hst. rewrite <- Hst.
-    match goal with [ Hst : make_guard ?T _ = _ |- _ ] => set (test1 := T) end.
-    destruct (eval_test env test1) eqn:Htest1.
-    + exists (eval_expr env lb). exists (eval_expr env ub).
-      rewrite make_guard_correct, Htest1.
-      split.
-      * split.
-        -- intros Hsem; inversion_clear Hsem; auto.
-        -- intros Hsem; constructor; auto.
-      * intros x. rewrite find_bounds_correct; [|exact Hlb|exact Hub|exact Henvlen].
-        unfold test1 in Htest1. rewrite make_poly_test_correct in Htest1 by auto.
-        unfold in_poly in *. rewrite forallb_forall. rewrite forallb_forall in Htest1.
-        split.
-        -- intros H c Hc Hcnth; apply H; auto.
-        -- intros H c Hc. destruct (nth n (fst c) 0 =? 0) eqn:Hcnth; reflect.
-           ++ simpl; erewrite satisfies_constraint_nth_zero_eq; rewrite ?rev_length; [|eauto|eauto].
-              apply Htest1. rewrite filter_In; reflect; auto.
-           ++ apply H; auto.
-    + exists 0. exists 0. rewrite make_guard_correct, Htest1. split.
-      * split.
-        -- intros H; rewrite H. econstructor; lia.
-        -- intros H; inversion_clear H; reflexivity.
-      * unfold test1 in Htest1. intros x. split; [|lia].
-        intros H; unfold in_poly in H; rewrite forallb_forall in H.
-        exfalso; eapply eq_true_false_abs; [|exact Htest1].
-        rewrite make_poly_test_correct by auto. unfold in_poly; rewrite forallb_forall.
-        intros c Hc; rewrite filter_In in Hc; destruct Hc as [Hcin Hcnth].
-        specialize (H c Hcin). reflect. simpl in H.
-        erewrite satisfies_constraint_nth_zero_eq in H; rewrite ?rev_length; eauto.
-Qed.
-
-Fixpoint polyloop_to_loop n pstmt : imp stmt :=
-  match pstmt with
-  | PSkip => pure (Seq nil)
-  | PSeq s1 s2 =>
-    BIND u1 <- polyloop_to_loop n s1 -;
-    BIND u2 <- polyloop_to_loop n s2 -;
-    pure (Seq (u1 :: u2 :: nil))
-  | PInstr i es =>
-    pure (Instr i (map (fun e => make_div (make_affine_expr n (snd e)) (Zpos (fst e))) es))
-  | PLoop pol inner =>
-    BIND inner1 <- polyloop_to_loop (S n) inner -;
-    scan_dimension n inner1 pol
-  | PGuard pol inner =>
-    BIND inner1 <- polyloop_to_loop n inner -;
-    pure (make_guard (make_poly_test n pol) inner1)
-  end.
-
-Lemma polyloop_to_loop_correct :
-  forall pstmt n env mem1 mem2,
-    WHEN st <- polyloop_to_loop n pstmt THEN
-    loop_semantics st env mem1 mem2 ->
-    length env = n ->
-    poly_loop_semantics pstmt env mem1 mem2.
-Proof.
-  induction pstmt; intros n env mem1 mem2 st Hst Hsem Henv; simpl in *.
-  - bind_imp_destruct Hst inner Hinner.
-    generalize (scan_dimension_sem _ _ _ _ Hst _ mem1 mem2 Henv).
-    intros [lb [ub [H1 H2]]].
-    econstructor; [exact H2|]. rewrite H1 in Hsem.
-    eapply iter_semantics_map; [|exact Hsem].
-    intros x mem3 mem4 Hx Hsem2. simpl in Hsem2. eapply IHpstmt; simpl; eauto.
-  - apply mayReturn_pure in Hst. rewrite <- Hst in *.
-    inversion_clear Hsem. constructor.
-    rewrite map_map in H.
-    unfold eval_affine_expr. erewrite map_ext; [exact H|].
-    intros [k a]; simpl. rewrite make_div_correct, make_affine_expr_correct by auto. reflexivity.
-  - apply mayReturn_pure in Hst. rewrite <- Hst in *.
-    inversion_clear Hsem. econstructor; auto.
-  - bind_imp_destruct Hst u1 Hu1. bind_imp_destruct Hst u2 Hu2.
-    apply mayReturn_pure in Hst; rewrite <- Hst in *.
-    inversion_clear Hsem; inversion_clear H0. replace mem2 with mem4 by (inversion_clear H2; auto).
-    econstructor; [eapply IHpstmt1|eapply IHpstmt2]; eauto.
-  - bind_imp_destruct Hst inner Hinner. apply mayReturn_pure in Hst; rewrite <- Hst in *.
-    rewrite make_guard_correct in Hsem.
-    rewrite make_poly_test_correct in Hsem by auto.
-    destruct (in_poly (rev env) p) eqn:Htest.
-    + apply PLGuardTrue; [|auto]. eapply IHpstmt; eauto.
-    + rewrite Hsem; apply PLGuardFalse; auto.
-Qed.
 
 Fixpoint generate_loop (d : nat) (n : nat) (pi : Polyhedral_Instruction) : imp poly_stmt :=
   match d with
@@ -808,7 +395,6 @@ Fixpoint mymap {A B : Type} (f : A -> B) (l : list A) : list B :=
 
 Definition mapM {A B : Type} (f : A -> imp B) (l : list A) : imp (list B) := sequence (mymap f l).
 
-(* meh *)
 Lemma Forall2_mymap_left :
   forall (A B C : Type) (R : B -> C -> Prop) (f : A -> B) xs ys, Forall2 R (mymap f xs) ys <-> Forall2 (fun x y => R (f x) y) xs ys.
 Proof.
@@ -868,50 +454,6 @@ Lemma mapM_length :
 Proof.
   intros A B f xs ys H; apply sequence_length in H; rewrite mymap_length in H; auto.
 Qed.
-
-(*
-(* sigh *)
-Fixpoint mycombine {A B : Type} (xs : list A) (ys : list B) :=
-  match xs, ys with
-  | x :: xs, y :: ys => (x, y) :: mycombine xs ys
-  | _, _ => nil
-  end.
-
-Lemma mymap_mycombine :
-  forall (A B : Type) (xs : list A) (ys : list B), length xs = length ys -> mymap fst (mycombine xs ys) = xs.
-Proof.
-  intros A B. induction xs.
-  - intros ys H; destruct ys; simpl in *; congruence.
-  - intros ys H; destruct ys; simpl in *; [|rewrite IHxs]; congruence.
-Qed.
-
-Lemma iter_semantics_mycombine :
-  forall (A B : Type) P (xs : list A) (ys : list B) mem1 mem2,
-    length xs = length ys -> iter_semantics P xs mem1 mem2 <-> iter_semantics (fun p => P (fst p)) (mycombine xs ys) mem1 mem2.
-Proof.
-  intros A B P xs ys mem1 mem2 H.
-  replace xs with (mymap fst (mycombine xs ys)) at 1 by (apply mymap_mycombine; auto).
-  rewrite iter_semantics_mymapl; reflexivity.
-Qed.
-
-Lemma iter_semantics_sequence_rev :
-  forall (A : Type) P (xs : list (imp A)) (ys : list A) mem1 mem2,
-    mayReturn (sequence xs) ys ->
-    iter_semantics P ys mem1 mem2 ->
-    iter_semantics (fun '(x, y) mem3 mem4 => mayReturn x y /\ P y mem3 mem4) (mycombine xs ys) mem1 mem2.
-Proof.
-  intros A P. induction xs.
-  - intros ys mem1 mem2 Hys Hsem; simpl in *. apply mayReturn_pure in Hys; rewrite <- Hys in Hsem.
-    inversion_clear Hsem; constructor.
-  - intros ys mem1 mem2 Hys Hsem; simpl in *.
-    bind_imp_destruct Hys y Hy.
-    bind_imp_destruct Hys ys1 Hys1.
-    apply mayReturn_pure in Hys; rewrite <- Hys in *.
-    inversion_clear Hsem.
-    econstructor; [eauto|].
-    apply IHxs; auto.
-Qed.
-*)
 
 Lemma mapM_in_iff :
   forall (A B : Type) (f : A -> imp B) (xs : list A) (y : B),
@@ -1088,77 +630,6 @@ Definition dummy_pi := {|
   pi_transformation := nil ;
   pi_schedule := nil
 |}.
-
-Definition check_toposort cstr out :=
-  if Permutation_dec _ Nat.eq_dec (n_range (length cstr)) out then
-    forallb (fun k2 => forallb (fun k1 => negb (nth (nth k2 out 0%nat) (nth (nth k1 out 0%nat) cstr nil) true)) (n_range k2)) (n_range (length cstr))
-  else
-    Debugging.failwith Debugging.CERT "topo_sort: not permutation" false.
-
-Lemma check_toposort_correct_permutation :
-  forall cstr out, check_toposort cstr out = true -> Permutation (n_range (length cstr)) out.
-Proof.
-  intros cstr out H. unfold check_toposort in H.
-  unfold Debugging.failwith in *.
-  destruct Permutation_dec; [auto|congruence].
-Qed.
-
-Lemma check_toposort_correct_sorted :
-  forall cstr out, check_toposort cstr out = true ->
-              forall k1 k2, (k1 < k2 < length cstr)%nat -> nth (nth k2 out 0%nat) (nth (nth k1 out 0%nat) cstr nil) true = false.
-Proof.
-  intros cstr out H k1 k2 [Hk1 Hk2].
-  unfold check_toposort, Debugging.failwith in H. destruct Permutation_dec; [|congruence].
-  rewrite <- negb_true_iff. 
-  rewrite forallb_forall in H. rewrite <- n_range_in in Hk2.
-  specialize (H k2 Hk2); rewrite forallb_forall in H. rewrite <- n_range_in in Hk1.
-  apply H; auto.
-Qed.
-
-Definition topo_sort cstr :=
-  BIND out <- topo_sort_untrusted cstr -;
-  if check_toposort cstr out then
-    pure out
-  else
-    Debugging.failwith Debugging.CERT "topo_sort: not good sort" (alarm "topo_sort verification failed" out).
-
-Lemma topo_sort_permutation :
-  forall cstr, WHEN out <- topo_sort cstr THEN Permutation (n_range (length cstr)) out.
-Proof.
-  intros cstr out Hout.
-  bind_imp_destruct Hout out1 Hout1.
-  destruct (check_toposort cstr out1) eqn:Hcheck.
-  - apply mayReturn_pure in Hout; rewrite Hout in *. apply check_toposort_correct_permutation; auto.
-  - apply mayReturn_alarm in Hout; tauto.
-Qed.
-
-Lemma topo_sort_sorted :
-  forall cstr, WHEN out <- topo_sort cstr THEN forall k1 k2, (k1 < k2 < length cstr)%nat ->
-               nth (nth k2 out 0%nat) (nth (nth k1 out 0%nat) cstr nil) true = false.
-Proof.
-  intros cstr out Hout.
-  bind_imp_destruct Hout out1 Hout1.
-  destruct (check_toposort cstr out1) eqn:Hcheck.
-  - apply mayReturn_pure in Hout; rewrite Hout in *. apply check_toposort_correct_sorted; auto.
-  - apply mayReturn_alarm in Hout; tauto.
-Qed.
-
-
-Lemma topo_sort_indices_correct :
-  forall cstr, WHEN out <- topo_sort cstr THEN forall i, In i out -> (i < length cstr)%nat.
-Proof.
-  intros cstr out Hout i Hin.
-  rewrite <- n_range_in.
-  eapply Permutation_in; [symmetry; apply topo_sort_permutation|]; eauto.
-Qed.
-
-Lemma topo_sort_length :
-  forall cstr, WHEN out <- topo_sort cstr THEN length out = length cstr.
-Proof.
-  intros cstr out Hout.
-  erewrite Permutation_length; [|symmetry; eapply topo_sort_permutation; eauto].
-  rewrite n_range_length; eauto.
-Qed.
 
 Fixpoint poly_difference p1 p2 :=
   match p2 with
