ImpureAlarmConfig.v
@@ -1,3 +1,4 @@
+Require Import Result.
 Require Import Vpl.Impure.
 Require Vpl.ImpureConfig.
 
@@ -6,3 +7,18 @@ Export CoreAlarmed.
 
 Ltac bind_imp_destruct H id1 id2 :=
   apply CoreAlarmed.Base.mayReturn_bind in H; destruct H as [id1 [id2 H]].
+
+Definition res_to_alarm {A : Type} (d : A) (x : result A) : imp A :=
+  match x with
+  | Ok a => pure a
+  | Err s => alarm s d
+  end.
+
+Lemma res_to_alarm_correct :
+  forall (A : Type) (d : A) (x : result A) (y : A),
+    mayReturn (res_to_alarm d x) y -> x = Ok y.
+Proof.
+  intros A d x y. destruct x; simpl.
+  - intros H. f_equal. apply mayReturn_pure. auto.
+  - intros H. apply mayReturn_alarm in H. tauto.
+Qed.
