Instr.v
@@ -1,32 +1,10 @@
 Require Import ZArith.
 Require Import List.
 
-Open Scope Z_scope.
+Require Import Semantics.
 
 (** * The basic instructions and their semantics *)
 
 Parameter instr : Type.
 Parameter dummy_instr : instr.
-
-Parameter mem : Type.
 Parameter instr_semantics : instr -> list Z -> mem -> mem -> Prop.
-
-(** * Iterating semantics on a list *)
-
-Inductive iter_semantics {A : Type} (P : A -> mem -> mem -> Prop) : list A -> mem -> mem -> Prop :=
-| IDone : forall mem, iter_semantics P nil mem mem
-| IProgress : forall x l mem1 mem2 mem3,
-    P x mem1 mem2 -> iter_semantics P l mem2 mem3 ->
-    iter_semantics P (x :: l) mem1 mem3.
-
-Lemma iter_semantics_map {A : Type} (P Q : A -> mem -> mem -> Prop) :
-  forall l mem1 mem2,
-    (forall x mem1 mem2, In x l -> P x mem1 mem2 -> Q x mem1 mem2) ->
-    iter_semantics P l mem1 mem2 ->
-    iter_semantics Q l mem1 mem2.
-Proof.
-  intros l mem1 mem2 Himp Hsem.
-  induction Hsem; econstructor; eauto; [eapply Himp|eapply IHHsem]; eauto.
-  - simpl; auto.
-  - intros; apply Himp; simpl; auto.
-Qed.
