LoopGen.v
@@ -1,0 +1,420 @@
+Require Import ZArith.
+Require Import List.
+Require Import Bool.
+Require Import Psatz.
+Require Import Setoid Morphisms.
+Require Import Permutation.
+
+Require Import Linalg.
+Require Import Loop.
+Require Import PolyLoop.
+Require Import Misc.
+Require Import Semantics.
+Require Import Instr.
+Require Import VplInterface.
+Require Import Result.
+Require Import Heuristics.
+
+Require Import Vpl.Impure.
+Require Import ImpureAlarmConfig.
+
+Open Scope Z_scope.
+Open Scope list_scope.
+
+(** * Creating expressions that evaluate to a given linear function *)
+
+Fixpoint make_linear_expr (n : nat) (l : list Z) :=
+  match n, l with
+  | O, _ | _, nil => Constant 0
+  | S n, x :: l => make_sum (make_mult x (Var n)) (make_linear_expr n l)
+  end.
+
+Theorem make_linear_expr_correct_aux :
+  forall n l env, (length env >= n)%nat -> eval_expr env (make_linear_expr n l) = dot_product l (rev (firstn n env)).
+Proof.
+  induction n.
+  - intros l env Hel. destruct env; destruct l; simpl in *; auto; lia.
+  - intros l env Hel.
+    destruct l as [|x l]; simpl in Hel; destruct (rev (firstn (S n) env)) as [|y ev] eqn:Hrev; auto; simpl; auto.
+    + destruct env as [|e env]; simpl in *; [lia | destruct (rev (firstn n env)); simpl in *; congruence].
+    + rewrite firstn_nth_app with (d := 0) in Hrev by auto. rewrite rev_unit in Hrev.
+      injection Hrev as Hnth Hrev. rewrite make_sum_correct, make_mult_correct, IHn by lia; simpl. congruence.
+Qed.
+
+Theorem make_linear_expr_correct :
+  forall n l env, length env = n -> eval_expr env (make_linear_expr n l) = dot_product l (rev env).
+Proof.
+  intros. rewrite make_linear_expr_correct_aux by lia. f_equal. f_equal. apply firstn_all2. lia.
+Qed.
+
+Definition make_affine_expr (n : nat) (e : (list Z * Z)%type) := make_sum (make_linear_expr n (fst e)) (Constant (snd e)).
+
+Theorem make_affine_expr_correct :
+  forall n e env, length env = n -> eval_expr env (make_affine_expr n e) = dot_product (fst e) (rev env) + snd e.
+Proof.
+  intros. unfold make_affine_expr. rewrite make_sum_correct, make_linear_expr_correct; auto.
+Qed.
+
+(** * Creating upper and lower bounds for a given variable in a constraint *)
+
+Definition make_lower_bound n c :=
+  make_div (make_sum (Constant ((- nth n (fst c) 0) - 1)) (make_affine_expr n (fst c, -(snd c)))) (-(nth n (fst c) 0)).
+
+Lemma make_lower_bound_correct :
+  forall n c env x, length env = n -> nth n (fst c) 0 < 0 -> (eval_expr env (make_lower_bound n c) <= x <-> satisfies_constraint (rev env ++ x :: nil) c = true).
+Proof.
+  intros n c env x Hlen Hneg.
+  unfold satisfies_constraint. simpl.
+  reflect. unfold make_lower_bound; rewrite make_div_correct, make_sum_correct, make_affine_expr_correct by auto. simpl.
+  rewrite dot_product_app_left, dot_product_resize_right, dot_product_commutative.
+  rewrite rev_length, Hlen.
+  replace (dot_product (x :: nil) (skipn n (fst c))) with (x * nth n (fst c) 0) at 1;
+    [| transitivity (x * nth 0 (skipn n (fst c)) 0);
+       [ rewrite nth_skipn; f_equal; f_equal; lia
+       | destruct (skipn n (fst c)) as [|z l]; [|destruct l]; simpl; lia
+       ]
+    ].
+  rewrite div_le_iff by lia. nia.
+Qed.
+
+Definition make_upper_bound n c :=
+  make_div (make_sum (Constant (nth n (fst c) 0)) (make_affine_expr n (mult_vector (-1) (fst c), snd c))) (nth n (fst c) 0).
+
+Lemma make_upper_bound_correct :
+  forall n c env x, length env = n -> 0 < nth n (fst c) 0 -> (x < eval_expr env (make_upper_bound n c) <-> satisfies_constraint (rev env ++ x :: nil) c = true).
+Proof.
+  intros n c env x Hlen Hpos.
+  unfold satisfies_constraint. simpl.
+  reflect. unfold make_upper_bound; rewrite make_div_correct, make_sum_correct, make_affine_expr_correct by auto. simpl.
+  rewrite dot_product_mult_left.
+  rewrite dot_product_app_left, dot_product_resize_right, dot_product_commutative.
+  rewrite rev_length, Hlen.
+  replace (dot_product (x :: nil) (skipn n (fst c))) with (x * nth n (fst c) 0) at 1;
+    [| transitivity (x * nth 0 (skipn n (fst c)) 0);
+       [ rewrite nth_skipn; f_equal; f_equal; lia
+       | destruct (skipn n (fst c)) as [|z l]; [|destruct l]; simpl; lia
+       ]
+    ].
+  rewrite div_gt_iff by lia. nia.
+Qed.
+
+Opaque make_lower_bound make_upper_bound.
+
+(** * Finding the upper and lower bounds for a given variable of a polyhedron *)
+
+Fixpoint find_lower_bound_aux (e : option expr) (n : nat) (p : polyhedron) :=
+  match p with
+  | nil => match e with Some e => Ok e | None => Err "No lower bound found" end
+  | c :: p => if nth n (fst c) 0 <? 0 then
+               find_lower_bound_aux (Some (match e with Some e => make_max e (make_lower_bound n c) | None => make_lower_bound n c end)) n p
+             else
+               find_lower_bound_aux e n p
+  end.
+
+Lemma find_lower_bound_aux_correct :
+  forall n pol env x e lb, find_lower_bound_aux e n pol = Ok lb -> length env = n ->
+                      eval_expr env lb <= x <->
+                      ((match e with Some e => eval_expr env e <= x | None => True end) /\
+                       forall c, In c pol -> nth n (fst c) 0 < 0 -> satisfies_constraint (rev env ++ x :: nil) c = true).
+Proof.
+  intros n pol. induction pol.
+  - intros env x e lb Hlb Hlength. simpl in *.
+    destruct e; simpl in *; [|congruence].
+    injection Hlb as Hlb; rewrite Hlb.
+    split; intros H; tauto.
+  - intros env x e lb Hlb Hlen. simpl in *.
+    destruct (nth n (fst a) 0 <? 0) eqn:Hcmp.
+    + reflect. rewrite IHpol; eauto; simpl.
+      destruct e; simpl; [rewrite make_max_correct, Z.max_lub_iff|]; rewrite make_lower_bound_correct by auto; split.
+      * intros [[H1 H2] H3]. split; auto. intros c [Hce|Hcin] Hcnth; [congruence|auto].
+      * intros [H1 H2]. split; [split|]; auto.
+      * intros [H1 H2]. split; auto. intros c [Hce|Hcin] Hcnth; [congruence|auto].
+      * intros [H1 H2]. split; auto.
+    + reflect. rewrite IHpol; eauto; simpl. f_equiv. split.
+      * intros H c [Hce|Hcin] Hcnth; auto; rewrite Hce in *; lia.
+      * intros H c Hcin Hcnth; auto.
+Qed.
+
+Fixpoint find_upper_bound_aux (e : option expr) (n : nat) (p : polyhedron) :=
+  match p with
+  | nil => match e with Some e => Ok e | None => Err "No upper bound found" end
+  | c :: p => if 0 <? nth n (fst c) 0 then
+               find_upper_bound_aux (Some (match e with Some e => make_min e (make_upper_bound n c) | None => make_upper_bound n c end)) n p
+             else
+               find_upper_bound_aux e n p
+  end.
+
+Lemma find_upper_bound_aux_correct :
+  forall n pol env x e ub, find_upper_bound_aux e n pol = Ok ub -> length env = n ->
+                      x < eval_expr env ub <->
+                      ((match e with Some e => x < eval_expr env e | None => True end) /\
+                       forall c, In c pol -> 0 < nth n (fst c) 0 -> satisfies_constraint (rev env ++ x :: nil) c = true).
+Proof.
+  intros n pol. induction pol.
+  - intros env x e ub Hub Hlength. simpl in *.
+    destruct e; simpl in *; [|congruence].
+    injection Hub as Hub; rewrite Hub.
+    split; intros H; tauto.
+  - intros env x e lb Hub Hlen. simpl in *.
+    destruct (0 <? nth n (fst a) 0) eqn:Hcmp.
+    + reflect. rewrite IHpol; eauto; simpl.
+      destruct e; simpl; [rewrite make_min_correct, Z.min_glb_lt_iff|]; rewrite make_upper_bound_correct by auto; split.
+      * intros [[H1 H2] H3]. split; auto. intros c [Hce|Hcin] Hcnth; [congruence|auto].
+      * intros [H1 H2]. split; [split|]; auto.
+      * intros [H1 H2]. split; auto. intros c [Hce|Hcin] Hcnth; [congruence|auto].
+      * intros [H1 H2]. split; auto.
+    + reflect. rewrite IHpol; eauto; simpl. f_equiv. split.
+      * intros H c [Hce|Hcin] Hcnth; auto; rewrite Hce in *; lia.
+      * intros H c Hcin Hcnth; auto.
+Qed.
+
+Definition find_lower_bound := find_lower_bound_aux None.
+Definition find_upper_bound := find_upper_bound_aux None.
+
+Theorem find_lower_bound_correct :
+  forall n pol env x lb, find_lower_bound n pol = Ok lb -> length env = n ->
+                    eval_expr env lb <= x <-> (forall c, In c pol -> nth n (fst c) 0 < 0 -> satisfies_constraint (rev env ++ x :: nil) c = true).
+Proof.
+  intros n pol env x lb Hlb Hlen.
+  rewrite find_lower_bound_aux_correct by eauto. simpl. tauto.
+Qed.
+
+Theorem find_upper_bound_correct :
+  forall n pol env x ub, find_upper_bound n pol = Ok ub -> length env = n ->
+                    x < eval_expr env ub <-> (forall c, In c pol -> 0 < nth n (fst c) 0 -> satisfies_constraint (rev env ++ x :: nil) c = true).
+
+Proof.
+  intros n pol env x ub Hub Hlen.
+  rewrite find_upper_bound_aux_correct by eauto. simpl. tauto.
+Qed.
+
+Theorem find_bounds_correct :
+  forall n pol env x lb ub, find_lower_bound n pol = Ok lb -> find_upper_bound n pol = Ok ub -> length env = n ->
+                       eval_expr env lb <= x < eval_expr env ub <-> (forall c, In c pol -> nth n (fst c) 0 <> 0 -> satisfies_constraint (rev env ++ x :: nil) c = true).
+Proof.
+  intros n pol env x lb ub Hlb Hub Hlen.
+  rewrite find_lower_bound_correct; eauto.
+  rewrite find_upper_bound_correct; eauto.
+  split.
+  - intros [H1 H2] c Hin Hnotzero. destruct (nth n (fst c) 0 <=? 0) eqn:Hcmp; reflect; [apply H1 | apply H2]; auto; lia.
+  - intros H; split; intros c Hin Hcmp; apply H; auto; lia.
+Qed.
+
+
+Definition solve_eq n c :=
+  (make_div (make_affine_expr n (mult_vector (-1) (fst c), snd c)) (nth n (fst c) 0),
+   make_eq (make_mod (make_affine_expr n (mult_vector (-1) (fst c), snd c)) (nth n (fst c) 0)) (Constant 0)).
+
+Lemma solve_eq_correct :
+  forall n c env x, length env = n -> nth n (fst c) 0 <> 0 ->
+               (eval_expr env (fst (solve_eq n c)) = x /\ eval_test env (snd (solve_eq n c)) = true) <->
+                dot_product (rev env ++ x :: nil) (fst c) = snd c.
+Proof.
+  intros n c env x Hlen Hnz. simpl.
+  rewrite make_div_correct, make_eq_correct, make_mod_correct, !make_affine_expr_correct by auto. simpl.
+  rewrite !dot_product_mult_left, dot_product_app_left, dot_product_resize_right, dot_product_commutative.
+  rewrite rev_length, Hlen.
+  replace (dot_product (x :: nil) (skipn n (fst c))) with (x * nth n (fst c) 0) at 1;
+    [| transitivity (x * nth 0 (skipn n (fst c)) 0);
+       [ rewrite nth_skipn; f_equal; f_equal; lia
+       | destruct (skipn n (fst c)) as [|z l]; [|destruct l]; simpl; lia
+       ]
+    ].
+  reflect. split.
+  - intros [Hdiv Hmod]. rewrite <- Z.div_exact in Hmod by auto. nia.
+  - intros H. rewrite <- H, Z.add_assoc, Z.add_opp_diag_l, Z.add_0_l. split.
+    + apply Z.div_mul; auto.
+    + apply Z.mod_mul; auto.
+Qed.
+
+Definition make_affine_test n c := make_le (make_linear_expr n (fst c)) (Constant (snd c)).
+
+Lemma make_affine_test_correct :
+  forall env n c, length env = n -> eval_test env (make_affine_test n c) = satisfies_constraint (rev env) c.
+Proof.
+  intros. simpl in *. unfold make_affine_test. rewrite make_le_correct, make_linear_expr_correct; auto.
+  rewrite dot_product_commutative. reflexivity.
+Qed.
+
+Definition make_poly_test n poly :=
+  and_all (map (make_affine_test n) poly).
+
+Lemma make_poly_test_correct :
+  forall n poly env, length env = n ->
+                eval_test env (make_poly_test n poly) = in_poly (rev env) poly.
+Proof.
+  intros n poly env Hlen.
+  unfold make_poly_test. rewrite and_all_correct. unfold in_poly.
+  rewrite forallb_map. apply forallb_ext. intros c. apply make_affine_test_correct. auto.
+Qed.
+
+Definition scan_dimension (n : nat) (inner : stmt) (p : polyhedron) : imp stmt :=
+  match find_eq n p with
+  | Some c =>
+    let '(result, test) := solve_eq n c in
+    let cstrs := map (fun c1 => make_affine_test n (make_constraint_with_eq n c c1)) (filter (fun c => negb (nth n (fst c) 0 =? 0)) p) in
+    let cstrs1 := map (make_affine_test n) (filter (fun c => nth n (fst c) 0 =? 0) p) in
+    pure (make_guard (make_and test (and_all (cstrs ++ cstrs1))) (make_let result inner))
+  | None =>
+    BIND lb <- res_to_alarm (Constant 0) (find_lower_bound n p) -;
+    BIND ub <- res_to_alarm (Constant 0) (find_upper_bound n p) -;
+    let cstrs := filter (fun c => nth n (fst c) 0 =? 0) p in
+    pure (make_guard (make_poly_test n cstrs) (Loop lb ub inner))
+  end.
+
+
+Lemma dot_product_nth_zero_eval :
+  forall env n u x, nth n u 0 = 0 -> length env = n -> dot_product (env ++ x :: nil) u = dot_product env u.
+Proof.
+  intros env n u x H1 H2.
+  rewrite <- dot_product_assign_left_zero with (k := n) (s := 0) by auto.
+  rewrite assign_app_ge by lia. rewrite H2, Nat.sub_diag.
+  unfold assign. simpl.
+  f_equiv. rewrite <- app_nil_r. f_equiv.
+Qed.
+
+Lemma satisfies_constraint_nth_zero_eq :
+  forall env n c x, nth n (fst c) 0 = 0 -> length env = n -> satisfies_constraint (env ++ x :: nil) c = satisfies_constraint env c.
+Proof.
+  intros. unfold satisfies_constraint.
+  erewrite dot_product_nth_zero_eval; eauto.
+Qed.
+
+Lemma scan_dimension_sem :
+  forall n inner pol,
+    WHEN st <- scan_dimension n inner pol THEN
+         forall env mem1 mem2,
+           length env = n ->
+           exists lb ub,
+             (loop_semantics st env mem1 mem2 <-> iter_semantics (fun x => loop_semantics inner (x :: env)) (Zrange lb ub) mem1 mem2) /\
+             (forall x, in_poly (rev (x :: env)) pol = true <-> lb <= x < ub).
+Proof.
+  intros n inner pol st Hst env mem1 mem2 Henvlen.
+  unfold scan_dimension in Hst.
+  destruct (find_eq n pol) as [c|] eqn:Hfindeq.
+  - destruct (solve_eq n c) as [result test] eqn:Hsolve. apply mayReturn_pure in Hst; rewrite <- Hst.
+    match goal with [ Hst : make_guard ?T _ = _ |- _ ] => set (test1 := T) end.
+    assert (Hcnth : 0 < nth n (fst c) 0) by (eapply find_eq_nth; eauto).
+    destruct (eval_test env test1) eqn:Htest1.
+    + exists (eval_expr env result). exists (eval_expr env (Sum result (Constant 1))). split.
+      * split.
+        -- intros Hsem. rewrite make_guard_correct, Htest1 in Hsem. unfold make_let in Hsem. inversion_clear Hsem. auto.
+        -- intros Hsem. rewrite make_guard_correct, Htest1. unfold make_let. constructor; auto.
+      * intros x. simpl.
+        unfold test1 in Htest1. rewrite make_and_correct in Htest1; reflect.
+        rewrite and_all_correct in Htest1. destruct Htest1 as [Htest Hcstr].
+        rewrite forallb_app, andb_true_iff in Hcstr. destruct Hcstr as [Hcstr1 Hcstr2].
+        transitivity (eval_expr env (fst (solve_eq n c)) = x /\ eval_test env (snd (solve_eq n c)) = true); [|rewrite Hsolve; simpl; intuition lia].
+        rewrite solve_eq_correct by (auto || lia).
+        split.
+        -- intros H. unfold in_poly in H. rewrite forallb_forall in H.
+           eapply find_eq_correct_1; eauto.
+        -- intros H. unfold in_poly; rewrite forallb_forall. intros c1 Hc1in.
+           rewrite forallb_map, forallb_forall in Hcstr1, Hcstr2. specialize (Hcstr1 c1). specialize (Hcstr2 c1).
+           rewrite filter_In, make_affine_test_correct in Hcstr1, Hcstr2 by auto.
+           destruct (nth n (fst c1) 0 =? 0) eqn:Hc1nth; reflect.
+           ++ erewrite satisfies_constraint_nth_zero_eq; rewrite ?rev_length; eauto.
+           ++ rewrite <- make_constraint_with_eq_correct_1 with (n := n) (c1 := c) by (auto || lia).
+              erewrite satisfies_constraint_nth_zero_eq; rewrite ?rev_length; eauto.
+              apply make_constraint_with_eq_nth; lia.
+    + exists 0. exists 0. split.
+      * split.
+        -- intros Hsem. rewrite make_guard_correct, Htest1 in Hsem; rewrite Hsem. constructor; lia.
+        -- intros Hsem. rewrite make_guard_correct, Htest1. inversion_clear Hsem. reflexivity.
+      * split; [|lia]. intros H. exfalso.
+        enough (eval_test env test1 = true) by congruence.
+        unfold test1. rewrite make_and_correct, and_all_correct, forallb_app, !forallb_map. reflect.
+        unfold in_poly in H. rewrite forallb_forall in H.
+        assert (Heq : dot_product (rev (x :: env)) (fst c) = snd c) by (eapply find_eq_correct_1; eauto). simpl in Heq.
+        split; [|split].
+        -- rewrite <- solve_eq_correct in Heq; [|exact Henvlen|lia]. rewrite Hsolve in Heq; simpl in Heq; tauto.
+        -- rewrite forallb_forall. intros c1 Hc1in. rewrite filter_In in Hc1in. reflect.
+           rewrite make_affine_test_correct by auto. destruct Hc1in as [Hc1in Hc1n]. specialize (H c1 Hc1in).
+           rewrite <- make_constraint_with_eq_correct_1 with (n := n) (c1 := c) in H by (auto || lia).
+           simpl in H; erewrite satisfies_constraint_nth_zero_eq in H; rewrite ?rev_length; eauto.
+           apply make_constraint_with_eq_nth; lia.
+        -- rewrite forallb_forall. intros c1 Hc1in. rewrite filter_In in Hc1in. reflect.
+           rewrite make_affine_test_correct by auto. destruct Hc1in as [Hc1in Hc1n]. specialize (H c1 Hc1in).
+           simpl in H; erewrite satisfies_constraint_nth_zero_eq in H; rewrite ?rev_length; eauto.
+  - bind_imp_destruct Hst lb Hlb. apply res_to_alarm_correct in Hlb.
+    bind_imp_destruct Hst ub Hub. apply res_to_alarm_correct in Hub.
+    apply mayReturn_pure in Hst. rewrite <- Hst.
+    match goal with [ Hst : make_guard ?T _ = _ |- _ ] => set (test1 := T) end.
+    destruct (eval_test env test1) eqn:Htest1.
+    + exists (eval_expr env lb). exists (eval_expr env ub).
+      rewrite make_guard_correct, Htest1.
+      split.
+      * split.
+        -- intros Hsem; inversion_clear Hsem; auto.
+        -- intros Hsem; constructor; auto.
+      * intros x. rewrite find_bounds_correct; [|exact Hlb|exact Hub|exact Henvlen].
+        unfold test1 in Htest1. rewrite make_poly_test_correct in Htest1 by auto.
+        unfold in_poly in *. rewrite forallb_forall. rewrite forallb_forall in Htest1.
+        split.
+        -- intros H c Hc Hcnth; apply H; auto.
+        -- intros H c Hc. destruct (nth n (fst c) 0 =? 0) eqn:Hcnth; reflect.
+           ++ simpl; erewrite satisfies_constraint_nth_zero_eq; rewrite ?rev_length; [|eauto|eauto].
+              apply Htest1. rewrite filter_In; reflect; auto.
+           ++ apply H; auto.
+    + exists 0. exists 0. rewrite make_guard_correct, Htest1. split.
+      * split.
+        -- intros H; rewrite H. econstructor; lia.
+        -- intros H; inversion_clear H; reflexivity.
+      * unfold test1 in Htest1. intros x. split; [|lia].
+        intros H; unfold in_poly in H; rewrite forallb_forall in H.
+        exfalso; eapply eq_true_false_abs; [|exact Htest1].
+        rewrite make_poly_test_correct by auto. unfold in_poly; rewrite forallb_forall.
+        intros c Hc; rewrite filter_In in Hc; destruct Hc as [Hcin Hcnth].
+        specialize (H c Hcin). reflect. simpl in H.
+        erewrite satisfies_constraint_nth_zero_eq in H; rewrite ?rev_length; eauto.
+Qed.
+
+Fixpoint polyloop_to_loop n pstmt : imp stmt :=
+  match pstmt with
+  | PSkip => pure (Seq nil)
+  | PSeq s1 s2 =>
+    BIND u1 <- polyloop_to_loop n s1 -;
+    BIND u2 <- polyloop_to_loop n s2 -;
+    pure (Seq (u1 :: u2 :: nil))
+  | PInstr i es =>
+    pure (Instr i (map (fun e => make_div (make_affine_expr n (snd e)) (Zpos (fst e))) es))
+  | PLoop pol inner =>
+    BIND inner1 <- polyloop_to_loop (S n) inner -;
+    scan_dimension n inner1 pol
+  | PGuard pol inner =>
+    BIND inner1 <- polyloop_to_loop n inner -;
+    pure (make_guard (make_poly_test n pol) inner1)
+  end.
+
+Lemma polyloop_to_loop_correct :
+  forall pstmt n env mem1 mem2,
+    WHEN st <- polyloop_to_loop n pstmt THEN
+    loop_semantics st env mem1 mem2 ->
+    length env = n ->
+    poly_loop_semantics pstmt env mem1 mem2.
+Proof.
+  induction pstmt; intros n env mem1 mem2 st Hst Hsem Henv; simpl in *.
+  - bind_imp_destruct Hst inner Hinner.
+    generalize (scan_dimension_sem _ _ _ _ Hst _ mem1 mem2 Henv).
+    intros [lb [ub [H1 H2]]].
+    econstructor; [exact H2|]. rewrite H1 in Hsem.
+    eapply iter_semantics_map; [|exact Hsem].
+    intros x mem3 mem4 Hx Hsem2. simpl in Hsem2. eapply IHpstmt; simpl; eauto.
+  - apply mayReturn_pure in Hst. rewrite <- Hst in *.
+    inversion_clear Hsem. constructor.
+    rewrite map_map in H.
+    unfold eval_affine_expr. erewrite map_ext; [exact H|].
+    intros [k a]; simpl. rewrite make_div_correct, make_affine_expr_correct by auto. reflexivity.
+  - apply mayReturn_pure in Hst. rewrite <- Hst in *.
+    inversion_clear Hsem. econstructor; auto.
+  - bind_imp_destruct Hst u1 Hu1. bind_imp_destruct Hst u2 Hu2.
+    apply mayReturn_pure in Hst; rewrite <- Hst in *.
+    inversion_clear Hsem; inversion_clear H0. replace mem2 with mem4 by (inversion_clear H2; auto).
+    econstructor; [eapply IHpstmt1|eapply IHpstmt2]; eauto.
+  - bind_imp_destruct Hst inner Hinner. apply mayReturn_pure in Hst; rewrite <- Hst in *.
+    rewrite make_guard_correct in Hsem.
+    rewrite make_poly_test_correct in Hsem by auto.
+    destruct (in_poly (rev env) p) eqn:Htest.
+    + apply PLGuardTrue; [|auto]. eapply IHpstmt; eauto.
+    + rewrite Hsem; apply PLGuardFalse; auto.
+Qed.
