Semantics.v
@@ -1,0 +1,23 @@
+Require Import List.
+
+Parameter mem : Type.
+
+(** * Iterating semantics on a list *)
+
+Inductive iter_semantics {A : Type} (P : A -> mem -> mem -> Prop) : list A -> mem -> mem -> Prop :=
+| IDone : forall mem, iter_semantics P nil mem mem
+| IProgress : forall x l mem1 mem2 mem3,
+    P x mem1 mem2 -> iter_semantics P l mem2 mem3 ->
+    iter_semantics P (x :: l) mem1 mem3.
+
+Lemma iter_semantics_map {A : Type} (P Q : A -> mem -> mem -> Prop) :
+  forall l mem1 mem2,
+    (forall x mem1 mem2, In x l -> P x mem1 mem2 -> Q x mem1 mem2) ->
+    iter_semantics P l mem1 mem2 ->
+    iter_semantics Q l mem1 mem2.
+Proof.
+  intros l mem1 mem2 Himp Hsem.
+  induction Hsem; econstructor; eauto; [eapply Himp|eapply IHHsem]; eauto.
+  - simpl; auto.
+  - intros; apply Himp; simpl; auto.
+Qed.
